Checkpoint invariance proof for commit

src/program_proof/rsm/distx/inv_txnsys.v
@@ -4,17 +4,35 @@ From Perennial.program_proof.rsm.pure Require Import dual_lookup vslice.
 
 (** Global transaction-system invariant. *)
 
-Definition conflict_free (acts : list action) (txns : gmap nat dbmap) : Prop.
+Definition conflict_free (future : list action) (tmodcs : gmap nat dbmap) : Prop.
 Admitted.
 
-Definition conflict_past (acts_future acts_past : list action) (txns : gmap nat dbmap) : Prop.
+Definition conflict_past (past future : list action) (tmodas : gmap nat dbmap) : Prop.
 Admitted.
 
-Definition cmtd_impl_prep (resm : gmap nat txnres) (wrsm : gmap nat dbmap) :=
-  ∀ ts, match resm !! ts with
-        | Some (ResCommitted wrs) => wrsm !! ts = Some wrs
-        | _ => True
-        end.
+Lemma conflict_free_inv_commit_committed ts wrs future tmodcs :
+  tmodcs !! ts = None ->
+  head future = Some (ActCmt ts wrs) ->
+  conflict_free future tmodcs ->
+  conflict_free (tail future) tmodcs.
+Admitted.
+
+Lemma conflict_free_inv_commit ts wrs future tmodcs :
+  head future = Some (ActCmt ts wrs) ->
+  conflict_free future tmodcs ->
+  conflict_free (tail future) (delete ts tmodcs).
+Admitted.
+
+Lemma conflict_past_inv_commit ts wrs past future tmodas :
+  head future = Some (ActCmt ts wrs) ->
+  conflict_past past future tmodas ->
+  conflict_past past (tail future) tmodas.
+Admitted.
+
+Definition prophesied_or_committed (tid : nat) (wcmts wabts cmts : gset nat) :=
+  (tid ∈ cmts ∧ tid ∉ wcmts) ∨
+  (tid ∈ wabts ∧ tid ∉ cmts) ∨
+  (tid ∈ wcmts ∧ tid ∉ cmts).
 
 Definition res_to_tmod (res : txnres) :=
   match res with
@@ -24,6 +42,35 @@ Definition res_to_tmod (res : txnres) :=
 
 Definition resm_to_tmods (resm : gmap nat txnres) :=
   omap res_to_tmod resm.
+
+Definition lnrz_txns_destined
+  (tids : gset nat) (tmodcs tmodas : gmap nat dbmap) (resm : gmap nat txnres) :=
+  set_Forall
+    (λ tid, prophesied_or_committed tid (dom tmodcs) (dom tmodas) (dom (resm_to_tmods resm)))
+    tids.
+
+Lemma resm_to_tmods_insert_aborted resm ts :
+  resm !! ts = None ->
+  resm_to_tmods (<[ts := ResAborted]> resm) = resm_to_tmods resm.
+Proof.
+  intros Hresm.
+  apply map_eq. intros tsx.
+  rewrite 2!lookup_omap.
+  destruct (decide (tsx = ts)) as [-> | Hne]; last by rewrite lookup_insert_ne.
+  by rewrite lookup_insert Hresm.
+Qed.
+
+Lemma resm_to_tmods_insert_committed resm ts wrs :
+  resm_to_tmods (<[ts := ResCommitted wrs]> resm) = <[ts := wrs]> (resm_to_tmods resm).
+Proof.
+  apply map_eq. intros tsx.
+  destruct (decide (tsx = ts)) as [-> | Hne]; last first.
+  { rewrite lookup_insert_ne; last done.
+    by rewrite 2!lookup_omap lookup_insert_ne; last done.
+  }
+  rewrite lookup_insert.
+  by rewrite lookup_omap lookup_insert.
+Qed.
 
 Lemma vslice_resm_to_tmods_committed_absent resm ts wrs key :
   resm !! ts = Some (ResCommitted wrs) ->
@@ -76,15 +123,30 @@ Section inv.
   (* TODO: remove this once we have real defintions for resources. *)
   Implicit Type (γ : distx_names).
 
-  Definition all_prepared γ ts keys : iProp Σ :=
-    [∗ set] gid ∈ ptgroups keys, txnprep_prep γ gid ts.
+  Definition all_prepared γ ts wrs : iProp Σ :=
+    txnwrs_receipt γ ts wrs ∗
+    [∗ set] gid ∈ ptgroups (dom wrs), txnprep_prep γ gid ts.
 
   Definition some_aborted γ ts : iProp Σ :=
-    ∃ gid, txnprep_unprep γ gid ts.
+    ∃ gid wrs, txnprep_unprep γ gid ts ∗
+               txnwrs_receipt γ ts wrs ∗
+               ⌜gid ∈ ptgroups (dom wrs)⌝.
+
+  Lemma all_prepared_some_aborted_false γ ts wrs :
+    all_prepared γ ts wrs -∗
+    some_aborted γ ts -∗
+    ⌜False⌝.
+  Proof.
+    iIntros "[Hwrs Hps] Habt".
+    iDestruct "Habt" as (gid wrsa) "(Hnp & Hwrsa & %Hgid)".
+    iDestruct (txnwrs_receipt_agree with "Hwrs Hwrsa") as %->.
+    iDestruct (big_sepS_elem_of with "Hps") as "Hp"; first apply Hgid.
+    by iDestruct (txnprep_receipt_agree with "Hp Hnp") as %Hcontra.
+  Qed.
 
   Definition valid_res γ ts res : iProp Σ :=
     match res with
-    | ResCommitted wrs => all_prepared γ ts (dom wrs)
+    | ResCommitted wrs => all_prepared γ ts wrs
     | ResAborted => some_aborted γ ts
     end.
 
@@ -94,11 +156,13 @@ Section inv.
   Proof. destruct res; apply _. Qed.
 
   Definition txn_inv γ : iProp Σ :=
-    ∃ (ts : nat) (future past : list action)
+    ∃ (ts : nat) (tids : gset nat) (future past : list action)
       (tmodcs tmodas : gmap nat dbmap)
       (resm : gmap nat txnres) (wrsm : gmap nat dbmap),
       (* global timestamp *)
       "Hts"    ∷ ts_auth γ ts ∗
+      (* linearized txns *)
+      "Htxnsl" ∷ txns_lnrz_auth γ tids ∗
       (* prophecy variable *)
       "Hproph" ∷ txn_proph γ future ∗
       (* transaction result map *)
@@ -110,11 +174,34 @@ Section inv.
       "Hkmodcs" ∷ ([∗ set] key ∈ keys_all, kmod_cmtd_half γ key (vslice (resm_to_tmods resm) key)) ∗
       (* safe commit/abort invariant *)
       "#Hvr"  ∷ ([∗ map] tid ↦ res ∈ resm, valid_res γ tid res) ∗
-      (* TODO: for coordinator recovery, add a monotonically growing set of
-      active txns; each active txn either appears in [txns_cmt]/[txns_abt] or in
-      the result map [resm]. *)
+      "%Hdest" ∷ ⌜lnrz_txns_destined tids tmodcs tmodas resm⌝ ∗
       "%Hcf"   ∷ ⌜conflict_free future tmodcs⌝ ∗
-      "%Hcp"   ∷ ⌜conflict_past future past tmodas⌝ ∗
-      "%Hcip"  ∷ ⌜cmtd_impl_prep resm wrsm⌝.
+      "%Hcp"   ∷ ⌜conflict_past past future tmodas⌝.
+
+  Definition txn_inv_no_future γ future : iProp Σ :=
+    ∃ (ts : nat) (tids : gset nat) (past : list action)
+      (tmodcs tmodas : gmap nat dbmap)
+      (resm : gmap nat txnres) (wrsm : gmap nat dbmap),
+      (* global timestamp *)
+      "Hts"    ∷ ts_auth γ ts ∗
+      (* linearized txns *)
+      "Htxnsl" ∷ txns_lnrz_auth γ tids ∗
+      (* transaction result map *)
+      "Hresm" ∷ txnres_auth γ resm ∗
+      (* transaction write set map *)
+      "Hwrsm" ∷ txnwrs_auth γ wrsm ∗
+      (* key modifications *)
+      "Hkmodls" ∷ ([∗ set] key ∈ keys_all, kmod_lnrz_half γ key (vslice tmodcs key)) ∗
+      "Hkmodcs" ∷ ([∗ set] key ∈ keys_all, kmod_cmtd_half γ key (vslice (resm_to_tmods resm) key)) ∗
+      (* safe commit/abort invariant *)
+      "#Hvr"  ∷ ([∗ map] tid ↦ res ∈ resm, valid_res γ tid res) ∗
+      "%Hdest" ∷ ⌜lnrz_txns_destined tids tmodcs tmodas resm⌝ ∗
+      "%Hcf"   ∷ ⌜conflict_free future tmodcs⌝ ∗
+      "%Hcp"   ∷ ⌜conflict_past past future tmodas⌝.
+
+  Lemma txn_inv_extract_future γ :
+    txn_inv γ -∗
+    ∃ future, txn_proph γ future ∗ txn_inv_no_future γ future.
+  Proof. iIntros "Htxn". iNamed "Htxn". iFrame "∗ # %". Qed.
 
 End inv.
