src/program_proof/rsm/distx/invariance/commit.v
@@ -1,12 +1,22 @@
 From Perennial.program_proof.rsm.distx Require Import prelude.
 
+Lemma resm_to_tmods_lookup_Some resm ts wrs :
+  resm_to_tmods resm !! ts = Some wrs ->
+  resm !! ts = Some (ResCommitted wrs).
+Proof.
+  intros Hresm.
+  rewrite /resm_to_tmods lookup_omap in Hresm.
+  destruct (resm !! ts) as [res |] eqn:Hres; last done.
+  by destruct res as [wrsx |] eqn:Hwrsx; first inv Hresm.
+Qed.
+
 Section inv.
   Context `{!distx_ghostG Σ}.
 
   (**
    * The commit action modifies the following logical states in [txn_inv]:
    * 1. Result map [resm].
-   * 2. Will-commit transaction map [txns_cmt].
+   * 2. Will-commit transaction map [tmodcs].
    * 3. Key modification map by committed txns [kmodcs].
    * 4. Key modification map by linearized txns [kmodls].
    * Invariants to re-establish:
@@ -30,15 +40,50 @@ Section inv.
    * prepared-implies-linearized-or-finalized.
    *)
 
-  Lemma txn_inv_commit γ ts wrs :
-    txnwrs_receipt γ ts wrs -∗
-    all_prepared γ ts (dom wrs) -∗
-    txn_inv γ -∗
+  Lemma txn_inv_commit γ tid wrs future :
+    head future = Some (ActCmt tid wrs) ->
+    txns_lnrz_receipt γ tid -∗
+    all_prepared γ tid wrs -∗
+    txn_inv_no_future γ future -∗
     ([∗ set] key ∈ keys_all, key_inv γ key) ==∗
-    txn_inv γ ∗
+    txn_inv_no_future γ (tail future) ∗
     ([∗ set] key ∈ keys_all, key_inv γ key) ∗
-    txnres_cmt γ ts wrs.
+    txnres_cmt γ tid wrs.
   Proof.
+    iIntros (Hhead) "#Htid #Hprep Htxnsys Hkeys".
+    iNamed "Htxnsys".
+    iDestruct (txns_lnrz_elem_of with "Htxnsl Htid") as %Htid.
+    apply Hdest in Htid as Hcases.
+    destruct Hcases as [[Hin Hnotin] | Hcases].
+    { (* Case: Txn [tid] has already aborted or committed. *)
+      rewrite elem_of_dom in Hin.
+      destruct Hin as [wrsc Hwrs].
+      apply resm_to_tmods_lookup_Some in Hwrs.
+      iDestruct (big_sepM_lookup with "Hvr") as "#Hres"; first apply Hwrs.
+      iAssert (⌜wrsc = wrs⌝)%I as %->.
+      { iDestruct "Hres" as "[Hwrsc _]".
+        iDestruct "Hprep" as "[Hwrs _]".
+        by iDestruct (txnwrs_receipt_agree with "Hwrs Hwrsc") as %?.
+      }
+      (* Case: Txn [tid] has already committed. Extract a witness without any update. *)
+      iDestruct (txnres_witness with "Hresm") as "#Hcmt"; first apply Hwrs.
+      unshelve epose proof (conflict_free_inv_commit_committed _ _ _ _ _ Hhead Hcf) as Hcf'.
+      { apply not_elem_of_dom_1, Hnotin. }
+      unshelve epose proof (conflict_past_inv_commit _ _ _ _ _ Hhead Hcp) as Hcp'.
+      by iFrame "∗ # %".
+    }
+    destruct Hcases as [[Htmodas Hnotin] | [Htmodcs Hnotin]].
+    { (* Case: Txn [tid] predicted to abort. Contradiction. *)
+      (* Case A: [tid] not showing at all in [future] -> contradicting [Hhead]. *)
+      (* Case B: [(tid, wrs)] conflicting with prior action -> add txnsys invs
+      ReadLength and CommitLength and key inv constraining the length of
+      replicated history with prepare timestamp. To show that [tid] is not
+      committed nor aborted, we use [Hnotin] for the former, and
+      [all_prepared_some_aborted_false] for the later. *)
+      (* Case C: [(tid, wrs)] does not satisfy [P wrs]. Contradiction with
+      additional premise. *)
+      admit.
+    }
   Admitted.
 
 End inv.
